theories/buffer.v
@@ -1,0 +1,56 @@
+From iris.heap_lang Require Export lang.
+From iris.proofmode Require Import tactics.
+From iris.algebra Require Import excl auth.
+From iris.base_logic.lib Require Import auth.
+Set Default Proof Using "Type".
+
+(* Buffer CMRA *)
+Definition buff_type := list val.
+
+Definition buffUR : ucmraT :=
+  optionUR (exclR (leibnizC (buff_type))).
+
+Definition to_buff (b : buff_type) : buffUR :=
+  Excl' (b: leibnizC buff_type).
+
+Class buffG (Σ :gFunctors) := BuffG {
+  buffG_authG :> authG Σ buffUR;
+}.
+
+Definition buffΣ : gFunctors :=
+  #[GFunctor (authR buffUR)].
+
+Instance subG_buffG {Σ} :
+  subG buffΣ Σ → buffG Σ.
+Proof. solve_inG. Qed.
+
+Section buff.
+  Context `{!buffG Σ} (N : namespace).
+
+  Lemma excl_eq γ x y :
+      own γ (● to_buff y) -∗ own γ (◯  to_buff x) -∗ ⌜x = y⌝%I.
+  Proof.
+    iIntros "Hauth Hfrag".
+    iDestruct (own_valid_2 with "Hauth Hfrag") as %Hvalid.
+    apply auth_valid_discrete_2 in Hvalid.
+    destruct Hvalid as [Hincl _].
+    apply Excl_included in Hincl.
+    unfold to_buff.
+    rewrite Hincl.
+    iFrame.
+    eauto.
+  Qed.
+
+  Lemma excl_update γ x y z :
+      own γ (● to_buff y) -∗ own γ (◯  to_buff x) -∗ |==> own γ (● to_buff z) ∗ own γ (◯  to_buff z).
+  Proof.
+    iIntros "Hauth Hfrag".
+    iDestruct (own_update_2 with "Hauth Hfrag") as "H".
+    { eapply (auth_update _ _ (to_buff z) (to_buff z)).
+      eapply option_local_update.
+      eapply exclusive_local_update. done. }
+    rewrite own_op.
+    done.
+  Qed.
+
+End buff.
